wip

theories/LambdaCalculus/Krivine.v
@@ -1,6 +1,8 @@
 (* 
   Problem(s):
     Krivine machine halting (KrivineM_HALT)
+    Krivine machine halting for closed terms (KrivineMclosed_HALT)
+    
 
   Literature:
     [1] Krivine, Jean-Louis.
@@ -12,6 +14,9 @@
 
 Require Undecidability.L.L.
 Import L (term, var, app, lam).
+
+Require Undecidability.LambdaCalculus.wCBN.
+Import wCBN (subst).
 
 (* (closure ctx t) is a lambda-term t in the environment ctx *)
 Inductive eterm := closure : list eterm -> term -> eterm.
@@ -38,3 +43,7 @@ Inductive halt_cbn : list eterm -> list eterm -> term -> Prop :=
 (* Krivine machine halting *)
 Definition KrivineM_HALT : term -> Prop :=
   fun t => halt_cbn nil nil t.
+
+(* Krivine machine halting for closed terms *)
+Definition KrivineMclosed_HALT : { t : term | forall sigma, subst sigma t = t } -> Prop :=
+  fun '(exist _ t _) => KrivineM_HALT t.
