theories/LambdaCalculus/Krivine_undec.v
@@ -7,15 +7,24 @@ From Undecidability.Synthetic Require Import Undecidability.
 
 Require Import Undecidability.LambdaCalculus.Krivine.
 From Undecidability.LambdaCalculus.Reductions Require
-  wCBNclosed_to_KrivineM_HALT.
+  wCBNclosed_to_KrivineMclosed_HALT.
 
 Require Import Undecidability.LambdaCalculus.wCBN_undec.
+
+(* Undecidability of Krivine machine halting for closed terms *)
+Theorem KrivineMclosed_HALT_undec : undecidable KrivineMclosed_HALT.
+Proof.
+  apply (undecidability_from_reducibility wCBNclosed_undec).
+  exact wCBNclosed_to_KrivineMclosed_HALT.reduction.
+Qed.
+
+Check KrivineMclosed_HALT_undec.
 
 (* Undecidability of Krivine machine halting *)
 Theorem KrivineM_HALT_undec : undecidable KrivineM_HALT.
 Proof.
-  apply (undecidability_from_reducibility wCBNclosed_undec).
-  exact wCBNclosed_to_KrivineM_HALT.reduction.
+  apply (undecidability_from_reducibility KrivineMclosed_HALT_undec).
+  exists (@proj1_sig L.term _). now intros [??].
 Qed.
 
 Check KrivineM_HALT_undec.
